Make MlirType a String (#121)
While this is not the end-goal with MlirType, it allows us to use it in
the parser and the printer, and allows us to catch some bugs in the
codebase that relied on the fact that all types are equal.

---------

Co-authored-by: Tobias Grosser <tobias@grosser.es>

Veir/IR/Basic.lean
@@ -30,7 +30,7 @@ instance : Hashable RegionPtr where
   hash regionPtr := hash regionPtr.id
 
 abbrev Location := Unit
-abbrev MlirType := Unit
+abbrev MlirType := String
 abbrev AttrDictionary := Unit
 
 /-
@@ -1249,7 +1249,7 @@ macro "setup_grind_with_get_set_definitions" : command => `(
   attribute [local grind cases] ValuePtr OpOperandPtr GenericPtr BlockOperandPtr OpResultPtr BlockArgumentPtr BlockOperandPtrPtr OpOperandPtrPtr
   attribute [local grind] OpOperandPtr.setNextUse OpOperandPtr.setBack OpOperandPtr.setOwner OpOperandPtr.setValue OpOperandPtr.set
   attribute [local grind] OpOperandPtrPtr.set OpOperandPtrPtr.get!
-  attribute [local grind] ValuePtr.getFirstUse! ValuePtr.getFirstUse ValuePtr.setFirstUse ValuePtr.setType
+  attribute [local grind] ValuePtr.getFirstUse! ValuePtr.getFirstUse ValuePtr.setFirstUse ValuePtr.setType ValuePtr.getType ValuePtr.getType!
   attribute [local grind] OpResultPtr.get! OpResultPtr.setFirstUse OpResultPtr.set OpResultPtr.setType
   attribute [local grind] BlockArgumentPtr.get! BlockArgumentPtr.setFirstUse BlockArgumentPtr.set BlockArgumentPtr.setType BlockArgumentPtr.setLoc
   attribute [local grind] OperationPtr.setOperands OperationPtr.setResults OperationPtr.pushResult OperationPtr.setRegions OperationPtr.setProperties  OperationPtr.pushOperand OperationPtr.allocEmpty OperationPtr.dealloc OperationPtr.setNextOp OperationPtr.setPrevOp OperationPtr.setParent OperationPtr.getNumResults! OperationPtr.getNumOperands! OperationPtr.getNumRegions! OperationPtr.getRegion! OperationPtr.getNumSuccessors! OperationPtr.set
